Characterize fallible functions

Tables/Table/Basic.lean
@@ -199,7 +199,7 @@ def ofRows (schema : Schema) (rows : Array Row) (h : ∀ row ∈ rows, row.schem
   }
 
 def ofRows? (rows : Array Row) : Except Error Table :=
-  if hsize : rows.size > 0 then
+  if hsize : 0 < rows.size then
     let schema := rows[0].schema
     let i := rows.findIdx (fun row => row.schema ≠ schema)
     if hi : i < rows.size then
@@ -381,30 +381,9 @@ def select (self : Table) (schema : Schema) (f : Row → (n : Nat) → n < self.
   }
 
 def select? (self : Table) (f : Row → (n : Nat) → n < self.nrows → Row) :
-    Except Error Table := do
-  if hsize : 0 < self.nrows then
-    let firstRow := f (self.getRow 0 hsize) 0 hsize
-    if hwf : firstRow.schema.Wf then
-      let table := ofRows firstRow.schema #[firstRow] (by simp) hwf
-      have hschema : table.schema = firstRow.schema := by
-        simp [table, ofRows, schema, Raw.ofRows_schema]
-
-      let result : { table : Table // table.schema = firstRow.schema } ← Nat.foldM (init := ⟨table, hschema⟩) self.nrows
-        fun i isLt table => do
-          if i = 0 then
-            -- Skip the first row, which is already added
-            return table
-          else
-            let row := f (self.getRow i isLt) i isLt
-            if h : row.schema = table.val.schema then
-              return ⟨table.val.addRow row h, by simp [addRow, schema, Raw.addRow_schema, table.property.symm]⟩
-            else
-              throw (.mismatchedSchema table.val.schema row.schema)
-      return result.val
-    else
-      throw .schemaNotWellFormed
-  else
-    .ok default
+    Except Error Table :=
+  let rows := Array.ofFn fun (i : Fin self.nrows) => f (self.getRow i i.isLt) i.val i.isLt
+  ofRows? rows
 
 def selectMany {α} (self : Table) (schema : Schema)
     (project : Row → (n : Nat) → n < self.nrows → Array α)
